Use concrete first-order terms from the AFP

Superposition_Calculus/Superposition.thy
@@ -5,8 +5,13 @@ theory Superposition
     "Saturation_Framework.Calculus"
     "Saturation_Framework.Lifting_to_Non_Ground_Calculi"
     "Saturation_Framework_Extensions.Clausal_Calculus"
-    "Abstract_Substitution_Extra"
+    "First_Order_Terms.Term"
+    "Knuth_Bendix_Order.Subterm_and_Context"
+
+    (* Theories from this formalization *)
+    "Abstract_Substitution_Extra_First_Order_Term"
 begin
+
 
 section \<open>Wellfounded_Extra\<close>
 
@@ -30,9 +35,9 @@ lemma wfP_lex_prodp: "wfP R\<^sub>A \<Longrightarrow> wfP R\<^sub>B \<Longrighta
 
 section \<open>Abstract Substitutions\<close>
 
-lemma (in substitution_ops)
+lemma (in substitution_ops) subst_cls_cong:
   assumes "\<And>L. L \<in># C \<Longrightarrow> atm_of L \<cdot>a \<sigma> = atm_of L \<cdot>a \<tau>"
-  shows subst_cls_cong: "subst_cls C \<sigma> = subst_cls C \<tau>"
+  shows "subst_cls C \<sigma> = subst_cls C \<tau>"
   unfolding subst_cls_def
 proof (rule multiset.map_cong0)
   fix L assume "L \<in># C"
@@ -43,67 +48,38 @@ proof (rule multiset.map_cong0)
 qed
 
 
-section \<open>Superposition Calculus\<close>
+section \<open>First_Order_Terms And Abstract_Substitution\<close>
 
-hide_type Inference_System.inference
-hide_const Inference_System.prems_of Inference_System.concl_of Inference_System.main_prem_of
+no_notation subst_compose (infixl "\<circ>\<^sub>s" 75)
+no_notation subst_apply_term (infixl "\<cdot>" 67)
 
-type_synonym 't atom = "'t \<times> 't"
+type_synonym ('f, 'v) atom = "('f, 'v) term \<times> ('f, 'v) term"
 
-locale superposition_calculus =
-  term_subst: basic_substitution subst_trm id_subst comp_subst
-  for
-    id_subst :: 's and
-    comp_subst :: "'s \<Rightarrow> 's \<Rightarrow> 's" and
-    subst_trm :: "'t \<Rightarrow> 's \<Rightarrow> 't" (infixl "\<cdot>t" 67) and
-    subst_trm_set :: "'t set \<Rightarrow> 's \<Rightarrow> 't set" (infixl "\<cdot>ts" 67)  +
-  fixes less_trm :: "'t \<Rightarrow> 't \<Rightarrow> bool" (infix "\<prec>\<^sub>t" 50)
-  assumes
-    transp_less_trm[simp]: "transp (\<prec>\<^sub>t)" and
-    wfP_less_trm[simp]: "wfP (\<prec>\<^sub>t)"
-begin
+abbreviation subst_atm :: "('f, 'v) atom \<Rightarrow> ('f, 'v) subst \<Rightarrow> ('f, 'v) atom" where
+  "subst_atm A \<sigma> \<equiv> map_prod (\<lambda>t. subst_apply_term t \<sigma>) (\<lambda>t. subst_apply_term t \<sigma>) A"
 
-abbreviation lesseq_trm (infix "\<preceq>\<^sub>t" 50) where
-  "lesseq_trm \<equiv> (\<prec>\<^sub>t)\<^sup>=\<^sup>="
+global_interpretation substitution_ops subst_atm Var subst_compose .
 
-abbreviation less_atm :: "'t atom \<Rightarrow> 't atom \<Rightarrow> bool" (infix "\<prec>\<^sub>a" 50) where
-  "less_atm \<equiv> lex_prodp (\<prec>\<^sub>t) (\<prec>\<^sub>t)"
-
-abbreviation lesseq_atm (infix "\<preceq>\<^sub>a" 50) where
-  "lesseq_atm \<equiv> (\<prec>\<^sub>a)\<^sup>=\<^sup>="
-
-abbreviation less_lit :: "'t atom literal \<Rightarrow> 't atom literal \<Rightarrow> bool" (infix "\<prec>\<^sub>l" 50) where
-  "less_lit \<equiv> Clausal_Logic.less_lit (\<prec>\<^sub>a)"
-
-abbreviation lesseq_lit (infix "\<preceq>\<^sub>l" 50) where
-  "lesseq_lit \<equiv> (\<prec>\<^sub>l)\<^sup>=\<^sup>="
-
-abbreviation less_cls :: "'t atom clause \<Rightarrow> 't atom clause \<Rightarrow> bool" (infix "\<prec>\<^sub>c" 50) where
-  "less_cls \<equiv> multp (\<prec>\<^sub>l)"
-
-abbreviation lesseq_cls (infix "\<preceq>\<^sub>c" 50) where
-  "lesseq_cls \<equiv> (\<prec>\<^sub>c)\<^sup>=\<^sup>="
-
-abbreviation subst_atm (infixl "\<cdot>a" 67) where
-  "subst_atm A \<sigma> \<equiv> map_prod (\<lambda>t. subst_trm t \<sigma>) (\<lambda>t. subst_trm t \<sigma>) A"
-
-interpretation substitution_ops "(\<cdot>a)" id_subst comp_subst .
-
+notation subst_apply_term (infixl "\<cdot>t" 67)
+notation subst_atm_abbrev (infixl "\<cdot>a" 67)
+notation subst_lit (infixl "\<cdot>l" 67)
 notation subst_cls (infixl "\<cdot>" 67)
+notation comp_subst_abbrev (infixl "\<odot>" 67)
 
-interpretation substitution "(\<cdot>a)" id_subst comp_subst
+
+interpretation substitution subst_atm Var subst_compose
 proof unfold_locales
-  show "\<And>A. A \<cdot>a id_subst = A"
+  show "\<And>A. A \<cdot>a Var = A"
     by (simp add: prod.map_ident)
 next
   show "\<And>A \<sigma> \<tau>. A \<cdot>a (\<sigma> \<odot> \<tau>) = A \<cdot>a \<sigma> \<cdot>a \<tau>"
     by (simp add: prod.map_comp comp_def)
 next
   show "\<And>\<sigma> \<tau>. (\<And>A. A \<cdot>a \<sigma> = A \<cdot>a \<tau>) \<Longrightarrow> \<sigma> = \<tau>"
-    by (rule term_subst.subst_ext) force
+    by (rule subst_term_eqI) force
 next
-  fix C :: "'t atom clause" and \<sigma> :: 's
-  define T :: "'t set" where
+  fix C :: "('f, 'v) atom clause" and \<sigma> :: "('f, 'v) subst"
+  define T :: "('f, 'v) term set" where
     "T = (\<Union>L \<in> set_mset C. {fst (atm_of L), snd (atm_of L)})"
 
   assume ground_C_\<sigma>: "is_ground_cls (subst_cls C \<sigma>)"
@@ -117,7 +93,8 @@ next
       unfolding T_def by auto
 
     from \<open>L \<in># C\<close> have "is_ground_lit (subst_lit L \<sigma>)"
-      using ground_C_\<sigma> is_ground_cls_def multi_member_split by fastforce
+      using ground_C_\<sigma> is_ground_cls_def multi_member_split
+      by (metis (mono_tags, lifting) subst_cls_add_mset union_single_eq_member)
     hence "is_ground_atm (subst_atm (atm_of L) \<sigma>)"
       by (simp add: is_ground_lit_def)
     then show "term_subst.is_ground t'"
@@ -150,23 +127,64 @@ next
     qed
   qed
 qed
-      
+
+
+section \<open>Superposition Calculus\<close>
+
+hide_type Inference_System.inference
+hide_const Inference_System.prems_of Inference_System.concl_of Inference_System.main_prem_of
+
+locale superposition_calculus =
+  fixes less_trm :: "('f, 'v) term \<Rightarrow> ('f, 'v) term \<Rightarrow> bool" (infix "\<prec>\<^sub>t" 50)
+  assumes
+    transp_less_trm[simp]: "transp (\<prec>\<^sub>t)" and
+    wfP_less_trm[simp]: "wfP (\<prec>\<^sub>t)"
+begin
+
+abbreviation lesseq_trm (infix "\<preceq>\<^sub>t" 50) where
+  "lesseq_trm \<equiv> (\<prec>\<^sub>t)\<^sup>=\<^sup>="
+
+abbreviation less_atm :: "('f, 'v) atom \<Rightarrow> ('f, 'v) atom \<Rightarrow> bool" (infix "\<prec>\<^sub>a" 50) where
+  "less_atm \<equiv> lex_prodp (\<prec>\<^sub>t) (\<prec>\<^sub>t)"
+
+abbreviation lesseq_atm (infix "\<preceq>\<^sub>a" 50) where
+  "lesseq_atm \<equiv> (\<prec>\<^sub>a)\<^sup>=\<^sup>="
+
+abbreviation less_lit :: "('f, 'v) atom literal \<Rightarrow> ('f, 'v) atom literal \<Rightarrow> bool" (infix "\<prec>\<^sub>l" 50) where
+  "less_lit \<equiv> Clausal_Logic.less_lit (\<prec>\<^sub>a)"
+
+abbreviation lesseq_lit (infix "\<preceq>\<^sub>l" 50) where
+  "lesseq_lit \<equiv> (\<prec>\<^sub>l)\<^sup>=\<^sup>="
+
+abbreviation less_cls :: "('f, 'v) atom clause \<Rightarrow> ('f, 'v) atom clause \<Rightarrow> bool" (infix "\<prec>\<^sub>c" 50) where
+  "less_cls \<equiv> multp (\<prec>\<^sub>l)"
+
+abbreviation lesseq_cls (infix "\<preceq>\<^sub>c" 50) where
+  "lesseq_cls \<equiv> (\<prec>\<^sub>c)\<^sup>=\<^sup>="
+
 
 section \<open>Rules\<close>
 
 
-inductive superposition :: "'t atom clause \<Rightarrow> 't atom clause \<Rightarrow> 't atom clause \<Rightarrow> bool" where
+inductive superposition ::
+  "('f, 'v) atom clause \<Rightarrow> ('f, 'v) atom clause \<Rightarrow> ('f, 'v) atom clause \<Rightarrow> bool"
+where
   superpositionI: "
     \<not> (P\<^sub>2 \<preceq>\<^sub>c P\<^sub>1) \<Longrightarrow>
     P\<^sub>1 = add_mset L\<^sub>1 P\<^sub>1' \<Longrightarrow>
     P\<^sub>2 = add_mset L\<^sub>2 P\<^sub>2' \<Longrightarrow>
     (\<forall>L \<in># add_mset L\<^sub>1 P\<^sub>1'. \<not> (L\<^sub>1 \<preceq>\<^sub>l L)) \<Longrightarrow>
     (\<forall>L \<in># add_mset L\<^sub>2 P\<^sub>2'. \<not> (L\<^sub>1 \<preceq>\<^sub>l L)) \<Longrightarrow>
+    \<P> \<in> {Pos, Neg} \<Longrightarrow>
+    L\<^sub>1 = \<P> (s\<^sub>1\<langle>u\<^sub>1\<rangle>, s\<^sub>1') \<or> L\<^sub>2 = \<P> (s\<^sub>1', s\<^sub>1\<langle>u\<rangle>) \<Longrightarrow>
     L\<^sub>2 = Pos (t\<^sub>2, t\<^sub>2') \<or> L\<^sub>2 = Pos (t\<^sub>2', t\<^sub>2) \<Longrightarrow>
+    \<not> (s\<^sub>1\<langle>u\<^sub>1\<rangle> \<preceq>\<^sub>t s\<^sub>1') \<Longrightarrow>
     \<not> (t\<^sub>2 \<preceq>\<^sub>t t\<^sub>2') \<Longrightarrow>
+    term_subst.is_imgu \<mu> {{u\<^sub>1, t\<^sub>2}} \<Longrightarrow>
+    C = add_mset (\<P> (s\<^sub>1\<langle>t\<^sub>2\<rangle>, s\<^sub>1')) (P\<^sub>1' + P\<^sub>2') \<cdot> \<mu> \<Longrightarrow>
     superposition P\<^sub>1 P\<^sub>2 C"
 
-inductive eq_resolution :: "'t atom clause \<Rightarrow> 't atom clause \<Rightarrow> bool" where
+inductive eq_resolution :: "('f, 'v) atom clause \<Rightarrow> ('f, 'v) atom clause \<Rightarrow> bool" where
   eq_resolutionI: "
     P = add_mset L P' \<Longrightarrow>
     L = Neg (t\<^sub>1, t\<^sub>2) \<Longrightarrow>
@@ -174,7 +192,7 @@ inductive eq_resolution :: "'t atom clause \<Rightarrow> 't atom clause \<Righta
     C = P' \<cdot> \<mu> \<Longrightarrow>
     eq_resolution P C"
 
-inductive eq_factoring :: "'t atom clause \<Rightarrow> 't atom clause \<Rightarrow> bool" where
+inductive eq_factoring :: "('f, 'v) atom clause \<Rightarrow> ('f, 'v) atom clause \<Rightarrow> bool" where
   eq_factoringI: "
     P = add_mset L\<^sub>1 (add_mset L\<^sub>2 P') \<Longrightarrow>
     (\<forall>L \<in># add_mset L\<^sub>2 P'. \<not> (L\<^sub>1 \<prec>\<^sub>l L)) \<Longrightarrow>
@@ -187,15 +205,77 @@ inductive eq_factoring :: "'t atom clause \<Rightarrow> 't atom clause \<Rightar
     eq_factoring P C"
 
 
+section \<open>Correctness\<close>
+
+lemma eq_resolution_preserves_groundness:
+  assumes ground_P: "is_ground_cls P" and step: "eq_resolution P C"
+  shows "is_ground_cls C"
+  using step
+proof (cases P C rule: eq_resolution.cases)
+  case (eq_resolutionI L P' t\<^sub>1 t\<^sub>2 \<mu>)
+  then show ?thesis
+    by (smt (verit, best) ground_P is_ground_cls_add_mset is_ground_subst_cls)
+qed
+
+lemma ground_correctness_eq_resolution:
+  assumes step: "eq_resolution P C" and ground_P: "is_ground_cls P"
+  shows "\<forall>I. refl I \<longrightarrow> I \<TTurnstile> P \<longrightarrow> I \<TTurnstile> C"
+  using step
+proof (cases P C rule: eq_resolution.cases)
+  case (eq_resolutionI L P' t\<^sub>1 t\<^sub>2 \<mu>)
+  with ground_P have "is_ground_atm (t\<^sub>1, t\<^sub>2)"
+    by (simp add: is_ground_cls_def is_ground_lit_def)
+  hence "term_subst.is_ground t\<^sub>1 \<and> term_subst.is_ground t\<^sub>2"
+    by (smt (verit, best) is_ground_subst_atm map_prod_simp prod.inject term_subst.is_ground_def)
+  hence "term_subst.is_ground_set {t\<^sub>1, t\<^sub>2}"
+    by (simp add: term_subst.is_ground_set_def)
+
+  moreover from \<open>term_subst.is_imgu \<mu> {{t\<^sub>1, t\<^sub>2}}\<close> have "term_subst.is_unifier \<mu> {t\<^sub>1, t\<^sub>2}"
+    by (simp add: term_subst.is_imgu_def term_subst.is_unifiers_def)
+
+  ultimately have "t\<^sub>1 = t\<^sub>2"
+    using term_subst.ball_eq_constant_if_unifier[of "{t\<^sub>2}" \<mu> t\<^sub>1]
+    by simp
+
+  show ?thesis
+  proof (intro allI impI)
+    fix I
+    assume "refl I" and "I \<TTurnstile> P"
+    then obtain K where "K \<in># P" and "I \<TTurnstile>l K"
+      by (auto simp: true_cls_def)
+    hence "K \<noteq> L"
+      by (metis \<open>refl I\<close> \<open>t\<^sub>1 = t\<^sub>2\<close> \<open>L = Neg (t\<^sub>1, t\<^sub>2)\<close> reflD true_lit_simps(2))
+    hence "K \<in># P'"
+      using \<open>K \<in># P\<close> \<open>P = add_mset L P'\<close>
+      by simp
+    hence "K \<in># P' \<cdot> \<mu>"
+      by (smt (verit, best) ground_P is_ground_cls_add_mset is_ground_subst_cls eq_resolutionI(1))
+    thus "I \<TTurnstile> C"
+      using \<open>C = P' \<cdot> \<mu>\<close> \<open>I \<TTurnstile>l K\<close>
+      by blast
+  qed
+qed
+
+lemma ground_correctness_eq_factoring:
+  assumes step: "eq_factoring P C" and ground_P: "is_ground_cls P"
+  shows "\<forall>I. refl I \<longrightarrow> I \<TTurnstile> P \<longrightarrow> I \<TTurnstile> C"
+  using step
+proof (cases P C rule: eq_factoring.cases)
+  case (eq_factoringI L\<^sub>1 L\<^sub>2 P' s\<^sub>1 t\<^sub>1 s\<^sub>2 t\<^sub>2 \<mu>)
+  then show ?thesis
+    sorry
+qed
+
+
 section \<open>Ground Layer\<close>
 
-abbreviation G_Inf :: "'t atom clause inference set" where
+abbreviation G_Inf :: "('f, 'v) atom clause inference set" where
   "G_Inf \<equiv> {}"
 
-abbreviation G_Bot :: "'t atom clause set" where
+abbreviation G_Bot :: "('f, 'v) atom clause set" where
   "G_Bot \<equiv> {{#}}"
 
-abbreviation G_entails :: "'t atom clause set \<Rightarrow> 't atom clause set \<Rightarrow> bool" where
+abbreviation G_entails :: "('f, 'v) atom clause set \<Rightarrow> ('f, 'v) atom clause set \<Rightarrow> bool" where
   "G_entails \<equiv> (\<TTurnstile>e)"
 
 interpretation G: sound_inference_system G_Inf G_Bot G_entails
@@ -237,24 +317,24 @@ qed
 section \<open>First-Order Layer\<close>
 
 
-abbreviation F_Inf :: "'t atom clause inference set" where
+abbreviation F_Inf :: "('f, 'v) atom clause inference set" where
   "F_Inf \<equiv> {}"
 
-abbreviation F_Bot :: "'t atom clause set" where
+abbreviation F_Bot :: "('f, 'v) atom clause set" where
   "F_Bot \<equiv> {{#}}"
 
-abbreviation F_entails :: "'t atom clause set \<Rightarrow> 't atom clause set \<Rightarrow> bool" where
+abbreviation F_entails :: "('f, 'v) atom clause set \<Rightarrow> ('f, 'v) atom clause set \<Rightarrow> bool" where
   "F_entails \<equiv> (\<TTurnstile>e)"
 
 typedecl Q
 
-definition \<G>_F :: "Q \<Rightarrow> 't atom clause \<Rightarrow> 't atom clause set" where
+definition \<G>_F :: "Q \<Rightarrow> ('f, 'v) atom clause \<Rightarrow> ('f, 'v) atom clause set" where
   "\<G>_F \<equiv> \<lambda>_ _. {}"
 
-definition \<G>_I :: "Q \<Rightarrow> 't atom clause inference \<Rightarrow> 't atom clause inference set option" where
+definition \<G>_I :: "Q \<Rightarrow> ('f, 'v) atom clause inference \<Rightarrow> ('f, 'v) atom clause inference set option" where
   "\<G>_I \<equiv> \<lambda>_ _. None"
 
-definition Prec_F :: "'t atom clause \<Rightarrow> 't atom clause \<Rightarrow> 't atom clause \<Rightarrow> bool" where
+definition Prec_F :: "('f, 'v) atom clause \<Rightarrow> ('f, 'v) atom clause \<Rightarrow> ('f, 'v) atom clause \<Rightarrow> bool" where
   "Prec_F \<equiv> \<lambda>_ _ _. False"
 
 interpretation F: lifting_intersection F_Inf G_Bot "UNIV :: Q set" "\<lambda>(_ :: Q). G_Inf"
@@ -274,6 +354,7 @@ qed
 interpretation F: sound_inference_system F_Inf F_Bot F.entails_\<G>
 proof unfold_locales
   show "\<And>\<iota>. \<iota> \<in> F_Inf \<Longrightarrow> F.entails_\<G> (set (prems_of \<iota>)) {concl_of \<iota>}"
+    unfolding F.entails_\<G>_def
     sorry
 qed
 
