Superposition_Calculus/Abstract_Substitution_Extra.thy
@@ -40,6 +40,21 @@ definition is_mgu :: "'s \<Rightarrow> 'x set set \<Rightarrow> bool" where
 definition is_imgu :: "'s \<Rightarrow> 'x set set \<Rightarrow> bool" where
   "is_imgu \<sigma> XX \<longleftrightarrow> is_unifiers \<sigma> XX \<and> (\<forall>\<tau>. is_unifiers \<tau> XX \<longrightarrow> \<tau> = \<sigma> \<odot> \<tau>)"
 
+lemma is_unifier_iff_if_finite:
+  assumes "finite X"
+  shows "is_unifier \<sigma> X \<longleftrightarrow> (\<forall>x\<in>X. \<forall>y\<in>X. x \<cdot> \<sigma> = y \<cdot> \<sigma>)"
+proof (rule iffI)
+  show "is_unifier \<sigma> X \<Longrightarrow> (\<forall>x\<in>X. \<forall>y\<in>X. x \<cdot> \<sigma> = y \<cdot> \<sigma>)"
+    using assms
+    unfolding is_unifier_def
+    by (metis One_nat_def card_le_Suc0_iff_eq finite_imageI image_eqI subst_set_def)
+next
+  show "(\<forall>x\<in>X. \<forall>y\<in>X. x \<cdot> \<sigma> = y \<cdot> \<sigma>) \<Longrightarrow> is_unifier \<sigma> X"
+    unfolding is_unifier_def
+    by (smt (verit, del_insts) One_nat_def basic_substitution_ops.subst_set_def card_eq_0_iff
+        card_le_Suc0_iff_eq dual_order.eq_iff imageE le_Suc_eq)
+qed
+
 end
 
 locale basic_substitution = basic_substitution_ops subst id_subst comp_subst for
@@ -66,6 +81,61 @@ subsection \<open>Associativity of Composition\<close>
 
 lemma comp_subst_assoc[simp]: "\<sigma> \<odot> (\<tau> \<odot> \<gamma>) = \<sigma> \<odot> \<tau> \<odot> \<gamma>"
   by (rule subst_ext) simp
+
+
+subsection \<open>Substituting on Ground Expression\<close>
+
+lemma is_ground_subst_ident[simp]: "is_ground x \<Longrightarrow> x \<cdot> \<sigma> = x"
+  unfolding is_ground_def by simp
+
+subsection \<open>Unifier of Ground Expressions\<close>
+
+lemma
+  assumes "is_unifier \<mu> {t\<^sub>1, t\<^sub>2}" and "is_ground t\<^sub>1" and "is_ground t\<^sub>2"
+  shows "t\<^sub>1 = t\<^sub>2"
+  using assms by (simp add: card_Suc_eq is_unifier_def le_Suc_eq subst_set_def)
+
+lemma is_unifier_subset: "is_unifier \<mu> A \<Longrightarrow> finite A \<Longrightarrow> B \<subseteq> A \<Longrightarrow> is_unifier \<mu> B"
+  by (smt (verit, best) card_mono dual_order.trans finite_imageI image_mono is_unifier_def
+      subst_set_def)
+
+lemma is_ground_set_subset: "is_ground_set A \<Longrightarrow> B \<subseteq> A \<Longrightarrow> is_ground_set B"
+  by (auto simp: is_ground_set_def)
+
+lemma ball_eq_constant_if_unifier:
+  assumes fin: "finite X" and unif: "is_unifier \<upsilon> (insert x X)" and "is_ground_set (insert x X)"
+  shows "\<forall>y \<in> X. y = x"
+  using assms
+proof (induction X rule: finite_induct)
+  case empty
+  show ?case by simp
+next
+  case (insert z F)
+
+  have "\<forall>y\<in>F. y = x"
+  proof (rule insert.IH)
+    show "is_unifier \<upsilon> (insert x F)"
+      using insert.hyps insert.prems(1)
+      by (auto elim: is_unifier_subset)
+  next
+    show "is_ground_set (insert x F)"
+      using insert.prems(2)
+      by (simp_all add: is_ground_set_def)
+  qed
+
+  moreover have "z = x"
+  proof -
+    have "x \<cdot> \<upsilon> = z \<cdot> \<upsilon>"
+      using insert.hyps insert.prems(1)
+      using is_unifier_iff_if_finite
+      by (meson finite.insertI insertCI)
+    then show ?thesis
+      by (metis is_ground_set_def insert.prems(2) insertCI is_ground_subst_ident)
+  qed
+
+  ultimately show ?case
+    by simp
+qed
 
 end
   
